well_formed_step for cesm

cbn_cem.v
@@ -2,40 +2,73 @@ Require cem cbn expr db relations.
 Require Import Unicode.Utf8 List NaryFunctions.
 Require Import expr_db util CpdtTactics.
 Require Import Basics.
+Require Import Compare_dec.
 
 Definition fresh (e : list nat) (h : cem.heap):= maximum (e ++ domain h). 
 
-(* Takes the closure from a configuration and converts it into the flattened
-configuration, so its free variables are pointing directly to the correct
-location*) 
-Definition closure_to_expr (c : cem.configuration) : option expr.tm 
-  := match c with | cem.conf h (cem.close t e') => let fix cte t e' e :=
-    match t with
-    | db.lam b => let f := fresh e h in 
-      match cte b e' (f :: e) with
-      | Some b' => Some (expr.abs f b')
-      | None => None
-      end
-    | db.var v => match nth_error e v with
-      | Some l => Some (expr.var l)
-      | None => match cem.clu v e' h with
-        | Some (l', _) => Some (expr.var l')
-        | None => None
-        end
-      end
-    | db.app m n => match cte m e' e with
-      | Some m' => match cte n e' e with 
-        | Some n' => Some (expr.app m' n')
-        | None => None
-        end
-      | None => None
-      end
+(* We define a term type with local and global variables to allow us to have an
+   equality relation between the cem and cbn configurations *)
+
+Inductive lgexpr := 
+  | gvar : nat → lgexpr
+  | lvar : nat → lgexpr
+  | lam : lgexpr → lgexpr
+  | app : lgexpr → lgexpr → lgexpr.
+
+(* Converting an exprssion to a local-global expr (lgexpr) translates bound
+variables to debruijn indices and free variables to unmodified global variable
+*)
+Fixpoint etolg (e : expr.tm) (env : Map nat nat) :=  match e with
+  | expr.abs v b => etolg b ((v, 0):: map (fmap S) env)
+  | expr.app m n => app (etolg m env) (etolg n env)
+  | expr.var v => match lookup v env with
+    | Some v' => lvar v'
+    | None => gvar v
     end
-    in cte t e' nil
+  end.
+ 
+Definition fmap_option {a b} : (a → b) → option a → option b := λ f o, 
+  match o with 
+  | Some m => Some (f m)
+  | None => None
   end.
 
+Definition seq_option {a b} : option (a → b) → option a → option b := λ f o,
+  match f, o with
+    | Some g, Some a => Some (g a)
+    | _, _ => None
+  end.
+  
+Notation "f <$> x" := (fmap_option f x) (at level 30).
+Notation "f <*> x" := (seq_option f x) (at level 40).
+
+(* Converting a debruijn term requires a full configuration, we don't change
+   local variables, and traverse the cactus stack to find the final location of the
+   closure corresponding to a variable and a cactus location *)
+Definition conftolg : cem.configuration → option lgexpr := λ c, match c with 
+  | cem.conf h (cem.close t e) => let fix cte t dep :=
+    match t with
+    | db.lam b => lam <$> cte b (S dep)
+    | db.app m n => app <$> cte m dep <*> cte n dep
+    | db.var v => if gt_dec dep v 
+      then Some (lvar v)
+      else (λ x, gvar (fst x)) <$> cem.clu (dep - v) e h
+    end in cte t 0
+  end.
 
 (*
+Lemma wf_conftolg : ∀ c, cem.well_formed c → ∃ e, conftolg c = Some e.
+intros. destruct c. destruct st_clos. generalize dependent clos_env. generalize
+dependent st_heap. induction clos_tm; intros.  simpl. simpl in H.
+destruct H. destruct H. destruct H. destruct H. destruct H. exists (gvar
+clos_env).  remember (lookup clos_env st_heap). destruct o. destruct c. simpl.
+reflexivity. unfold cem.clu in H. induction n. rewrite <- Heqo in H. inversion
+H.  rewrite <- Heqo in H. inversion H. simpl in H. destruct H.
+remember (db.fvs clos_tm). induction l. assert (map pred (remove 0 nil) = nil).
+reflexivity. rewrite H1 in H. rewrite Heql in H. specialize (IHclos_tm st_heap
+clos_env (conj H H0)). simpl. destruct IHclos_tm. simpl in H2. rewrite H2.   simpl in H. apply IHclos_tm. 
+Definition wf_closure_to_expr : {c | cem.well_formed c} → expr.tm := match 
+
 Definition flatten (c: {c | cem.well_formed c}) : cbn.configuration := match c with
   | exist (cem.conf h c) p => cbn.st (map (fmap (closure_to_expr ∘ cem.conf h ∘ cem.clclose) h))
                          (closure_to_expr nil h c)
